rename to motive

src/Init/Data/List/Lemmas.lean
@@ -750,22 +750,22 @@ Prove a proposition about the result of `List.foldl`,
 by proving it for the initial data,
 and the implication that the operation applied to any element of the list preserves the property.
 
-The motive `C` can take values in `Sort _`, so this may be used to construct data,
+The motive can take values in `Sort _`, so this may be used to construct data,
 as well as to prove propositions.
 -/
-def foldlRecOn {C : β → Sort _} : ∀ (l : List α) (op : β → α → β) (b : β) (_ : C b)
-    (_ : ∀ (b : β) (_ : C b) (a : α) (_ : a ∈ l), C (op b a)), C (List.foldl op b l)
+def foldlRecOn {motive : β → Sort _} : ∀ (l : List α) (op : β → α → β) (b : β) (_ : motive b)
+    (_ : ∀ (b : β) (_ : motive b) (a : α) (_ : a ∈ l), motive (op b a)), motive (List.foldl op b l)
   | [], _, _, hb, _ => hb
   | hd :: tl, op, b, hb, hl =>
     foldlRecOn tl op (op b hd) (hl b hb hd (mem_cons_self hd tl))
       fun y hy x hx => hl y hy x (mem_cons_of_mem hd hx)
 
-@[simp] theorem foldlRecOn_nil {C : β → Sort _} (hb : C b)
-    (hl : ∀ (b : β) (_ : C b) (a : α) (_ : a ∈ []), C (op b a)) :
+@[simp] theorem foldlRecOn_nil {motive : β → Sort _} (hb : motive b)
+    (hl : ∀ (b : β) (_ : motive b) (a : α) (_ : a ∈ []), motive (op b a)) :
     foldlRecOn [] op b hb hl = hb := rfl
 
-@[simp] theorem foldlRecOn_cons {C : β → Sort _} (hb : C b)
-    (hl : ∀ (b : β) (_ : C b) (a : α) (_ : a ∈ x :: l), C (op b a)) :
+@[simp] theorem foldlRecOn_cons {motive : β → Sort _} (hb : motive b)
+    (hl : ∀ (b : β) (_ : motive b) (a : α) (_ : a ∈ x :: l), motive (op b a)) :
     foldlRecOn (x :: l) op b hb hl =
       foldlRecOn l op (op b x) (hl b hb x (mem_cons_self x l))
         (fun b c a m => hl b c a (mem_cons_of_mem x m)) :=
@@ -776,22 +776,22 @@ Prove a proposition about the result of `List.foldr`,
 by proving it for the initial data,
 and the implication that the operation applied to any element of the list preserves the property.
 
-The motive `C` can take values in `Sort _`, so this may be used to construct data,
+The motive can take values in `Sort _`, so this may be used to construct data,
 as well as to prove propositions.
 -/
-def foldrRecOn {C : β → Sort _} : ∀ (l : List α) (op : α → β → β) (b : β) (_ : C b)
-    (_ : ∀ (b : β) (_ : C b) (a : α) (_ : a ∈ l), C (op a b)), C (List.foldr op b l)
+def foldrRecOn {motive : β → Sort _} : ∀ (l : List α) (op : α → β → β) (b : β) (_ : motive b)
+    (_ : ∀ (b : β) (_ : motive b) (a : α) (_ : a ∈ l), motive (op a b)), motive (List.foldr op b l)
   | nil, _, _, hb, _ => hb
   | x :: l, op, b, hb, hl =>
     hl (foldr op b l)
       (foldrRecOn l op b hb fun b c a m => hl b c a (mem_cons_of_mem x m)) x (mem_cons_self x l)
 
-@[simp] theorem foldrRecOn_nil {C : β → Sort _} (hb : C b)
-    (hl : ∀ (b : β) (_ : C b) (a : α) (_ : a ∈ []), C (op a b)) :
+@[simp] theorem foldrRecOn_nil {motive : β → Sort _} (hb : motive b)
+    (hl : ∀ (b : β) (_ : motive b) (a : α) (_ : a ∈ []), motive (op a b)) :
     foldrRecOn [] op b hb hl = hb := rfl
 
-@[simp] theorem foldrRecOn_cons {C : β → Sort _} (hb : C b)
-    (hl : ∀ (b : β) (_ : C b) (a : α) (_ : a ∈ x :: l), C (op a b)) :
+@[simp] theorem foldrRecOn_cons {motive : β → Sort _} (hb : motive b)
+    (hl : ∀ (b : β) (_ : motive b) (a : α) (_ : a ∈ x :: l), motive (op a b)) :
     foldrRecOn (x :: l) op b hb hl =
       hl _ (foldrRecOn l op b hb fun b c a m => hl b c a (mem_cons_of_mem x m))
         x (mem_cons_self x l) :=
